Proof for trunc1305

examples/low-level/crypto/Crypto.Symmetric.Poly1305.Lemmas.fst
@@ -487,46 +487,264 @@ let lemma_toField_1 s h n0 n1 n2 n3 =
   little_endian_append (Seq.append (Seq.append s04 s48) s812) s1216
 
 
-#reset-options "--initial_fuel 0 --max_fuel 0 --z3timeout 5"
+#reset-options "--initial_fuel 0 --max_fuel 0 --z3timeout 20"
 
-(* WIP *)
-assume val lemma_eval_5: h:HyperStack.mem -> a:Buffer.buffer U64.t{live h a /\ length a >= 5} ->
+val lemma_eval_5: h:HyperStack.mem -> a:Buffer.buffer U64.t{live h a /\ length a >= 5} ->
   Lemma (Crypto.Symmetric.Poly1305.Bigint.eval h a 5 =
     v (get h a 0) + pow2 26 * v (get h a 1) + pow2 52 * v (get h a 2) + pow2 78 * v (get h a 3)
     + pow2 104 * v (get h a 4))
+let lemma_eval_5 h a =
+  Crypto.Symmetric.Poly1305.Bigint.eval_def h a 5;
+  Crypto.Symmetric.Poly1305.Bigint.eval_def h a 4;
+  Crypto.Symmetric.Poly1305.Bigint.eval_def h a 3;
+  Crypto.Symmetric.Poly1305.Bigint.eval_def h a 2;
+  Crypto.Symmetric.Poly1305.Bigint.eval_def h a 1;
+  Crypto.Symmetric.Poly1305.Bigint.eval_def h a 0;
+  Crypto.Symmetric.Poly1305.Bigint.bitweight_def Crypto.Symmetric.Poly1305.Parameters.templ 4;
+  Crypto.Symmetric.Poly1305.Bigint.bitweight_def Crypto.Symmetric.Poly1305.Parameters.templ 3;
+  Crypto.Symmetric.Poly1305.Bigint.bitweight_def Crypto.Symmetric.Poly1305.Parameters.templ 2;
+  Crypto.Symmetric.Poly1305.Bigint.bitweight_def Crypto.Symmetric.Poly1305.Parameters.templ 1;
+  Crypto.Symmetric.Poly1305.Bigint.bitweight_def Crypto.Symmetric.Poly1305.Parameters.templ 0;
+  assert_norm (pow2 0 = 1)
 
-assume val lemma_little_endian_16: h:HyperStack.mem -> a:Buffer.buffer U8.t{live h a /\ length a = 16} ->
+#reset-options "--initial_fuel 0 --max_fuel 0 --z3timeout 20"
+
+
+val lemma_little_endian_16: h:HyperStack.mem -> a:Buffer.buffer U8.t{live h a /\ length a = 16} ->
   Lemma (let open FStar.UInt8 in
     little_endian (as_seq h a) =
             v (get h a 0) + pow2 8 * v (get h a 1) + pow2 16 * v (get h a 2) + pow2 24 * v (get h a 3)
   + pow2 32 * v (get h a 4) + pow2 40 * v (get h a 5) + pow2 48 * v (get h a 6) + pow2 56 * v (get h a 7)
   + pow2 64 * v (get h a 8) + pow2 72 * v (get h a 9) + pow2 80 * v (get h a 10) + pow2 88 * v (get h a 11)
   + pow2 96 * v (get h a 12) + pow2 104 * v (get h a 13) + pow2 112 * v (get h a 14) + pow2 120 * v (get h a 15) )
+let lemma_little_endian_16 h a =
+  let s = as_seq h a in
+  lemma_little_endian_from_top s;
+  lemma_little_endian_from_top_def s 16;
+  lemma_little_endian_from_top_def s 15;
+  lemma_little_endian_from_top_def s 14;
+  lemma_little_endian_from_top_def s 13;
+  lemma_little_endian_from_top_def s 12;
+  lemma_little_endian_from_top_def s 11;
+  lemma_little_endian_from_top_def s 10;
+  lemma_little_endian_from_top_def s 9;
+  lemma_little_endian_from_top_def s 8;
+  lemma_little_endian_from_top_def s 7;
+  lemma_little_endian_from_top_def s 6;
+  lemma_little_endian_from_top_def s 5;
+  lemma_little_endian_from_top_def s 4;
+  lemma_little_endian_from_top_def s 3;
+  lemma_little_endian_from_top_def s 2;
+  lemma_little_endian_from_top_def s 1;
+  lemma_little_endian_from_top_def s 0;
+  assert_norm (pow2 0 = 1)
 
-assume val lemma_trunc1305_0: a:U64.t -> Lemma
-  (v a % pow2 8 + pow2 8 * ((v a / pow2 8) % pow2 8) + pow2 16 * ((v a / pow2 16) % pow2 8) + pow2 24 * ((v a / pow2 24) % pow2 8)
+
+#reset-options "--initial_fuel 0 --max_fuel 0 --z3timeout 5"
+
+
+let lemma_mul_mod (a:nat) (b:pos) : Lemma ((b * a) % b = 0) = Math.Lemmas.lemma_mod_plus 0 a b
+
+
+val lemma_add_disjoint_bounded:
+  b0:nat -> b1:nat -> m:nat -> n:nat{n > m /\ n <= 64} ->
+  Lemma (requires ((b0 < pow2 m /\ b1 % pow2 m = 0 /\ b1 < pow2 n)))
+        (ensures  (b0 + b1 < pow2 n))
+let lemma_add_disjoint_bounded b0 b1 m n =
+  Math.Lemmas.lemma_div_mod b1 (pow2 m);
+  Math.Lemmas.lemma_mod_plus 0 b1 (pow2 m);
+  let c = b1 / pow2 m in
+  cut (c * pow2 m = b1);
+  cut ( (b1 + b0) = ((c*pow2 m) + b0));
+  lemma_div_pow2_lt b1 n m;
+  Math.Lemmas.pow2_plus (n-m) m;
+  cut ((c)*pow2 m + b0 < (pow2 (n-m)-1) * pow2 m + pow2 m)
+
+val lemma_trunc1305_0: a:U64.t -> Lemma
+  ((v a % pow2 8) + pow2 8 * ((v a / pow2 8) % pow2 8) + pow2 16 * ((v a / pow2 16) % pow2 8) + pow2 24 * ((v a / pow2 24) % pow2 8)
     = v a % pow2 32)
+let lemma_trunc1305_0 a =
+  assert_norm (pow2 0 = 1);
+  (* lemma_mul_mod ((v a / pow2 8) % pow2 8) (pow2 8); *)
+  (* Math.Lemmas.pow2_plus 8 8; *)
+  (* Math.Lemmas.pow2_plus 16 8; *)
+  (* lemma_add_disjoint_bounded (v a % pow2 8) (pow2 8 * ((v a / pow2 8) % pow2 8)) 8 16; *)
+  (* lemma_mul_mod ((v a / pow2 16) % pow2 8) (pow2 8); *)
+  (* lemma_add_disjoint_bounded ((v a % pow2 8) + pow2 8 * ((v a / pow2 8) % pow2 8)) *)
+  (*                            (pow2 16 * ((v a / pow2 16) % pow2 8)) 16 24; *)
+  (* lemma_mul_mod ((v a / pow2 24) % pow2 8) (pow2 8); *)
+  (* lemma_add_disjoint_bounded ((v a % pow2 8) + pow2 8 * ((v a / pow2 8) % pow2 8) + pow2 16 * ((v a / pow2 16) % pow2 8)) *)
+  (*                            (pow2 24 * ((v a / pow2 24) % pow2 8)) 24 32; *)
+   let va32 = v a % pow2 32 in
+   Math.Lemmas.pow2_modulo_modulo_lemma_1 (v a) 8 32;
+   Math.Lemmas.pow2_modulo_modulo_lemma_1 (v a) 16 32;
+   Math.Lemmas.pow2_modulo_modulo_lemma_1 (v a) 24 32;
+   Math.Lemmas.lemma_div_mod (va32) (pow2 24);
+   lemma_div_pow2_mod va32 32 24;
+   cut (va32 = pow2 24 * ((va32 / pow2 24) % pow2 8) + (va32 % pow2 24));
+   Math.Lemmas.lemma_div_mod (va32 % pow2 24) (pow2 16);
+   Math.Lemmas.pow2_modulo_division_lemma_1 va32 16 24;
+   Math.Lemmas.pow2_modulo_modulo_lemma_1 va32 16 24;
+   cut (va32 % pow2 24 = pow2 16 * ((va32/pow2 16)%pow2 8) + (va32 % pow2 16));
+   Math.Lemmas.lemma_div_mod (va32 % pow2 16) (pow2 8);
+   Math.Lemmas.pow2_modulo_division_lemma_1 va32 8 16;
+   Math.Lemmas.pow2_modulo_modulo_lemma_1 va32 8 16;
+   cut (va32 % pow2 16 = pow2 8 * ((va32/pow2 8)%pow2 8) + (va32 % pow2 8));
 
-assume val lemma_trunc1305_1: a:U64.t -> Lemma
-  ((v a * pow2 2) % pow2 8 + pow2 8 * ((v a / pow2 6) % pow2 8) + pow2 16 * ((v a / pow2 14) % pow2 8) + pow2 24 * ((v a / pow2 22) % pow2 8)
+  Math.Lemmas.pow2_modulo_division_lemma_1 (v a) 24 32;
+  cut (((v a % pow2 32) / pow2 24) % pow2 8 = (v a / pow2 24) % pow2 8);
+  Math.Lemmas.pow2_modulo_division_lemma_1 (v a) 16 32;
+  Math.Lemmas.pow2_modulo_modulo_lemma_1 (v a / pow2 16) 8 16;
+  cut (((v a % pow2 32) / pow2 16) % pow2 8 = (v a / pow2 16) % pow2 8);
+  Math.Lemmas.pow2_modulo_division_lemma_1 (v a) 8 32;
+  Math.Lemmas.pow2_modulo_modulo_lemma_1 (v a / pow2 8) 8 24;
+  cut (((v a % pow2 32) / pow2 8) % pow2 8 = (v a / pow2 8) % pow2 8)
+
+
+val lemma_trunc1305_1: a:U64.t -> Lemma
+  (((v a * pow2 2) % pow2 8) + pow2 8 * ((v a / pow2 6) % pow2 8) + pow2 16 * ((v a / pow2 14) % pow2 8) + pow2 24 * ((v a / pow2 22) % pow2 8)
     = pow2 2 * (v a % pow2 30))
+let lemma_trunc1305_1 a =
+  let va32 = ((v a * pow2 2) % pow2 32) in
+  Math.Lemmas.lemma_div_mod (va32) (pow2 24);
+  lemma_div_pow2_mod va32 32 24;
+  cut (va32 = pow2 24 * ((va32 / pow2 24) % pow2 8) + (va32 % pow2 24));
+  Math.Lemmas.pow2_modulo_division_lemma_1 (v a * pow2 2) 24 32;
+  cut (va32 / pow2 24 = ((v a * pow2 2) / pow2 24) % pow2 8);
+  Math.Lemmas.pow2_multiplication_division_lemma_2 (v a) 24 2;
+  cut ( (va32 / pow2 24) % pow2 8 = (v a / pow2 22) % pow2 8);
 
-assume val lemma_trunc1305_2: a:U64.t -> Lemma
-  ((v a * pow2 4) % pow2 8 + pow2 8 * ((v a / pow2 4) % pow2 8) + pow2 16 * ((v a / pow2 12) % pow2 8) + pow2 24 * ((v a / pow2 20) % pow2 8)
+  Math.Lemmas.lemma_div_mod (va32 % pow2 24) (pow2 16);
+  Math.Lemmas.pow2_modulo_division_lemma_1 va32 16 24;
+  Math.Lemmas.pow2_modulo_modulo_lemma_1 va32 16 24;
+  cut (va32 % pow2 24 = pow2 16 * ((va32/pow2 16)%pow2 8) + (va32 % pow2 16));
+
+  Math.Lemmas.pow2_modulo_division_lemma_1 (v a * pow2 2) 16 32;
+  cut (va32 / pow2 16 = ((v a * pow2 2) / pow2 16) % pow2 16);
+  Math.Lemmas.pow2_modulo_modulo_lemma_1 ((v a * pow2 2) / pow2 16) 8 16;
+  Math.Lemmas.pow2_multiplication_division_lemma_2 (v a) 16 2;
+  cut ( (va32 / pow2 16) % pow2 8 = (v a / pow2 14) % pow2 8);
+
+  Math.Lemmas.lemma_div_mod (va32 % pow2 16) (pow2 8);
+  Math.Lemmas.pow2_modulo_division_lemma_1 va32 8 16;
+  Math.Lemmas.pow2_modulo_modulo_lemma_1 va32 8 16;
+  cut (va32 % pow2 16 = pow2 8 * ((va32/pow2 8)%pow2 8) + (va32 % pow2 8));
+
+  Math.Lemmas.pow2_modulo_division_lemma_1 (v a * pow2 2) 8 32;
+  cut (va32 / pow2 8 = ((v a * pow2 2) / pow2 8) % pow2 24);
+  Math.Lemmas.pow2_modulo_modulo_lemma_1 ((v a * pow2 2) / pow2 8) 8 24;
+  Math.Lemmas.pow2_multiplication_division_lemma_2 (v a) 8 2;
+  cut ( (va32 / pow2 8) % pow2 8 = (v a / pow2 6) % pow2 8);
+
+  Math.Lemmas.pow2_modulo_modulo_lemma_1 (v a * pow2 2) 8 32;
+  Math.Lemmas.pow2_multiplication_modulo_lemma_2 (v a) 32 2
+
+
+val lemma_trunc1305_2: a:U64.t -> Lemma
+  (((v a * pow2 4) % pow2 8) + pow2 8 * ((v a / pow2 4) % pow2 8) + pow2 16 * ((v a / pow2 12) % pow2 8) + pow2 24 * ((v a / pow2 20) % pow2 8)
     = pow2 4 * (v a % pow2 28))
+let lemma_trunc1305_2 a =
+  let va32 = ((v a * pow2 4) % pow2 32) in
+  Math.Lemmas.lemma_div_mod (va32) (pow2 24);
+  lemma_div_pow2_mod va32 32 24;
+  cut (va32 = pow2 24 * ((va32 / pow2 24) % pow2 8) + (va32 % pow2 24));
+  Math.Lemmas.pow2_modulo_division_lemma_1 (v a * pow2 4) 24 32;
+  cut (va32 / pow2 24 = ((v a * pow2 4) / pow2 24) % pow2 8);
+  Math.Lemmas.pow2_multiplication_division_lemma_2 (v a) 24 4;
+  cut ( (va32 / pow2 24) % pow2 8 = (v a / pow2 20) % pow2 8);
 
-assume val lemma_trunc1305_3: a:U64.t -> Lemma
-  ((v a * pow2 6) % pow2 8 + pow2 8 * ((v a / pow2 2) % pow2 8) + pow2 16 * ((v a / pow2 10) % pow2 8) + pow2 24 * ((v a / pow2 18) % pow2 8)
+  Math.Lemmas.lemma_div_mod (va32 % pow2 24) (pow2 16);
+  Math.Lemmas.pow2_modulo_division_lemma_1 va32 16 24;
+  Math.Lemmas.pow2_modulo_modulo_lemma_1 va32 16 24;
+  cut (va32 % pow2 24 = pow2 16 * ((va32/pow2 16)%pow2 8) + (va32 % pow2 16));
+
+  Math.Lemmas.pow2_modulo_division_lemma_1 (v a * pow2 4) 16 32;
+  cut (va32 / pow2 16 = ((v a * pow2 4) / pow2 16) % pow2 16);
+  Math.Lemmas.pow2_modulo_modulo_lemma_1 ((v a * pow2 4) / pow2 16) 8 16;
+  Math.Lemmas.pow2_multiplication_division_lemma_2 (v a) 16 4;
+  cut ( (va32 / pow2 16) % pow2 8 = (v a / pow2 12) % pow2 8);
+
+  Math.Lemmas.lemma_div_mod (va32 % pow2 16) (pow2 8);
+  Math.Lemmas.pow2_modulo_division_lemma_1 va32 8 16;
+  Math.Lemmas.pow2_modulo_modulo_lemma_1 va32 8 16;
+  cut (va32 % pow2 16 = pow2 8 * ((va32/pow2 8)%pow2 8) + (va32 % pow2 8));
+
+  Math.Lemmas.pow2_modulo_division_lemma_1 (v a * pow2 4) 8 32;
+  cut (va32 / pow2 8 = ((v a * pow2 4) / pow2 8) % pow2 24);
+  Math.Lemmas.pow2_modulo_modulo_lemma_1 ((v a * pow2 4) / pow2 8) 8 24;
+  Math.Lemmas.pow2_multiplication_division_lemma_2 (v a) 8 4;
+  cut ( (va32 / pow2 8) % pow2 8 = (v a / pow2 4) % pow2 8);
+
+  Math.Lemmas.pow2_modulo_modulo_lemma_1 (v a * pow2 4) 8 32;
+  Math.Lemmas.pow2_multiplication_modulo_lemma_2 (v a) 32 4
+
+val lemma_trunc1305_3: a:U64.t -> Lemma
+  (((v a * pow2 6) % pow2 8) + pow2 8 * ((v a / pow2 2) % pow2 8) + pow2 16 * ((v a / pow2 10) % pow2 8) + pow2 24 * ((v a / pow2 18) % pow2 8)
     = pow2 6 * (v a % pow2 26))
+let lemma_trunc1305_3 a =
+  let va32 = ((v a * pow2 6) % pow2 32) in
+  Math.Lemmas.lemma_div_mod (va32) (pow2 24);
+  lemma_div_pow2_mod va32 32 24;
+  cut (va32 = pow2 24 * ((va32 / pow2 24) % pow2 8) + (va32 % pow2 24));
+  Math.Lemmas.pow2_modulo_division_lemma_1 (v a * pow2 6) 24 32;
+  cut (va32 / pow2 24 = ((v a * pow2 6) / pow2 24) % pow2 8);
+  Math.Lemmas.pow2_multiplication_division_lemma_2 (v a) 24 6;
+  cut ( (va32 / pow2 24) % pow2 8 = (v a / pow2 18) % pow2 8);
 
-assume val lemma_trunc1305_4: a:U64.t -> Lemma
-  (v a % pow2 8 + pow2 8 * ((v a / pow2 8) % pow2 8) + pow2 16 * ((v a / pow2 16) % pow2 8)
+  Math.Lemmas.lemma_div_mod (va32 % pow2 24) (pow2 16);
+  Math.Lemmas.pow2_modulo_division_lemma_1 va32 16 24;
+  Math.Lemmas.pow2_modulo_modulo_lemma_1 va32 16 24;
+  cut (va32 % pow2 24 = pow2 16 * ((va32/pow2 16)%pow2 8) + (va32 % pow2 16));
+
+  Math.Lemmas.pow2_modulo_division_lemma_1 (v a * pow2 6) 16 32;
+  cut (va32 / pow2 16 = ((v a * pow2 6) / pow2 16) % pow2 16);
+  Math.Lemmas.pow2_modulo_modulo_lemma_1 ((v a * pow2 6) / pow2 16) 8 16;
+  Math.Lemmas.pow2_multiplication_division_lemma_2 (v a) 16 6;
+  cut ( (va32 / pow2 16) % pow2 8 = (v a / pow2 10) % pow2 8);
+
+  Math.Lemmas.lemma_div_mod (va32 % pow2 16) (pow2 8);
+  Math.Lemmas.pow2_modulo_division_lemma_1 va32 8 16;
+  Math.Lemmas.pow2_modulo_modulo_lemma_1 va32 8 16;
+  cut (va32 % pow2 16 = pow2 8 * ((va32/pow2 8)%pow2 8) + (va32 % pow2 8));
+
+  Math.Lemmas.pow2_modulo_division_lemma_1 (v a * pow2 6) 8 32;
+  cut (va32 / pow2 8 = ((v a * pow2 6) / pow2 8) % pow2 24);
+  Math.Lemmas.pow2_modulo_modulo_lemma_1 ((v a * pow2 6) / pow2 8) 8 24;
+  Math.Lemmas.pow2_multiplication_division_lemma_2 (v a) 8 6;
+  cut ( (va32 / pow2 8) % pow2 8 = (v a / pow2 2) % pow2 8);
+
+  Math.Lemmas.pow2_modulo_modulo_lemma_1 (v a * pow2 6) 8 32;
+  Math.Lemmas.pow2_multiplication_modulo_lemma_2 (v a) 32 6
+
+val lemma_trunc1305_4: a:U64.t -> Lemma
+  ((v a % pow2 8) + pow2 8 * ((v a / pow2 8) % pow2 8) + pow2 16 * ((v a / pow2 16) % pow2 8)
     = v a % pow2 24)
+let lemma_trunc1305_4 a =
+   let va32 = v a % pow2 32 in
+   Math.Lemmas.pow2_modulo_modulo_lemma_1 (v a) 8 32;
+   Math.Lemmas.pow2_modulo_modulo_lemma_1 (v a) 16 32;
+   Math.Lemmas.pow2_modulo_modulo_lemma_1 (v a) 24 32;
+   Math.Lemmas.lemma_div_mod (va32) (pow2 24);
+   lemma_div_pow2_mod va32 32 24;
+   cut (va32 = pow2 24 * ((va32 / pow2 24) % pow2 8) + (va32 % pow2 24));
+   Math.Lemmas.lemma_div_mod (va32 % pow2 24) (pow2 16);
+   Math.Lemmas.pow2_modulo_division_lemma_1 va32 16 24;
+   Math.Lemmas.pow2_modulo_modulo_lemma_1 va32 16 24;
+   cut (va32 % pow2 24 = pow2 16 * ((va32/pow2 16)%pow2 8) + (va32 % pow2 16));
+   Math.Lemmas.lemma_div_mod (va32 % pow2 16) (pow2 8);
+   Math.Lemmas.pow2_modulo_division_lemma_1 va32 8 16;
+   Math.Lemmas.pow2_modulo_modulo_lemma_1 va32 8 16;
+   cut (va32 % pow2 16 = pow2 8 * ((va32/pow2 8)%pow2 8) + (va32 % pow2 8));
 
-assume val lemma_trunc1305_5: a0:U64.t -> a1:U64.t -> a2:U64.t -> a3:U64.t -> a4:U64.t -> Lemma
-  (requires (v a0 < pow2 26 /\ v a1 < pow2 26 /\ v a2 < pow2 26 /\ v a3 < pow2 26 /\ v a4 < pow2 26))
-  (ensures  ((v a0 + pow2 26 * v a1 + pow2 52 * v a2 + pow2 78 * v a3 + pow2 104 * v a4) % pow2 128
-    = (v a0 + pow2 26 * v a1 + pow2 52 * v a2 + pow2 78 * v a3 + pow2 104 * (v a4 % pow2 24)) ))
+  Math.Lemmas.pow2_modulo_division_lemma_1 (v a) 24 32;
+  cut (((v a % pow2 32) / pow2 24) % pow2 8 = (v a / pow2 24) % pow2 8);
+  Math.Lemmas.pow2_modulo_division_lemma_1 (v a) 16 32;
+  Math.Lemmas.pow2_modulo_modulo_lemma_1 (v a / pow2 16) 8 16;
+  cut (((v a % pow2 32) / pow2 16) % pow2 8 = (v a / pow2 16) % pow2 8);
+  Math.Lemmas.pow2_modulo_division_lemma_1 (v a) 8 32;
+  Math.Lemmas.pow2_modulo_modulo_lemma_1 (v a / pow2 8) 8 24;
+  cut (((v a % pow2 32) / pow2 8) % pow2 8 = (v a / pow2 8) % pow2 8)
+
 
 val lemma_norm_5:
   h:HyperStack.mem ->
@@ -536,11 +754,295 @@ val lemma_norm_5:
           /\ v (get h b 2) < pow2 26 /\ v (get h b 3) < pow2 26 /\ v (get h b 4) < pow2 26))
 let lemma_norm_5 h b = ()
 
-(* assume val lemma_trunc1305_6: a0:U64.t -> a1:U64.t -> a2:U64.t -> a3:U64.t -> a4:U64.t -> Lemma *)
-(*   (requires (v a0 < pow2 26 /\ v a1 < pow2 26 /\ v a2 < pow2 26 /\ v a3 < pow2 26 /\ v a4 < pow2 26)) *)
-(*   (ensures  ((v a0 + pow2 26 * v a1 + pow2 52 * v a2 + pow2 78 * v a3 + pow2 104 * v a4) *)
-(*     = v a0 % pow2 8 + ((v a0 / pow2 8) % pow2 8) + ((v a0 / pow2 16) % pow2 8) + ((v a0 / pow2 24) % pow2 8 *)
-(*       + pow2 2 *)
+
+#reset-options "--initial_fuel 0 --max_fuel 0 --z3timeout 20"
+
+val lemma_mod_sum_mul: x:nat -> y:nat -> l:nat -> m:nat -> Lemma
+  (requires (x % pow2 l = 0 /\ y < pow2 l /\ m >= l))
+  (ensures  ( (x + y) % pow2 m = x % pow2 m + y))
+let lemma_mod_sum_mul x y l m =
+  Math.Lemmas.lemma_mod_plus_distr_l x y (pow2 m);
+  cut ( (x + y) % pow2 m = (x % pow2 m + y) % pow2 m);
+  Math.Lemmas.lemma_div_mod x (pow2 l);
+  let c = x / pow2 l in
+  cut (c * pow2 l = x);
+  cut ( (x + y) % pow2 m = (((c*pow2 l)%pow2 m) + y) % pow2 m);
+  Math.Lemmas.pow2_multiplication_modulo_lemma_2 c m l;
+  cut ( (x + y) % pow2 m = (((c%pow2 (m-l))*pow2 l) + y) % pow2 m);
+  cut ( c % pow2 (m - l) < pow2 (m - l)); cut ((c%pow2 (m-l))*pow2 l + y < (pow2 (m-l)-1) * pow2 l + pow2 l);
+    Math.Lemmas.pow2_plus (m-l) l; Math.Lemmas.modulo_lemma (((c%pow2 (m-l))*pow2 l) + y) (pow2 m)
+
+
+#reset-options "--initial_fuel 0 --max_fuel 0 --z3timeout 20"
+
+let lemma_b3 (a0:U64.t{v a0 < pow2 26}) (a1:U64.t{v a1 < pow2 26}) : Lemma
+  (pow2 24 * (U8.v (uint64_to_uint8 ((a0 >>^ 24ul) |^ (a1 <<^ 2ul)))) = pow2 24 * ((v a0 / pow2 24) % pow2 8) + pow2 24 * ((v a1*pow2 2)%pow2 8))
+  = cut (v (a0 >>^ 24ul) = v a0 / pow2 24);
+    Math.Lemmas.pow2_multiplication_modulo_lemma_2 (v a1) 64 2;
+    Math.Lemmas.pow2_lt_compat 62 26; Math.Lemmas.modulo_lemma (v a1) (pow2 62);
+    Math.Lemmas.lemma_mod_plus 0 (v a1) (pow2 2);
+    lemma_div_pow2_lt (v a0) 26 24;
+    cut (v (a1 <<^ 2ul) % pow2 2 = 0);
+    cut (v (a0 >>^ 24ul) < pow2 2);
+    assert_norm(pow2 0 = 1);
+    Math.Lemmas.pow2_plus 26 2;
+    lemma_disjoint_bounded (a0 >>^ 24ul) (a1 <<^ 2ul) 0 2 28;
+    let r = U8.v (uint64_to_uint8 ((a0 >>^ 24ul) |^ (a1 <<^ 2ul))) in
+    cut (r = ((v a0 / pow2 24) + (v a1 * pow2 2)) % pow2 8);
+    lemma_mod_sum_mul (v a1 * pow2 2) (v a0 / pow2 24) 2 8
+
+
+let lemma_b6 (a1:U64.t{v a1 < pow2 26}) (a2:U64.t{v a2 < pow2 26}) : Lemma
+  (pow2 48 * (U8.v (uint64_to_uint8 ((a1 >>^ 22ul) |^ (a2 <<^ 4ul)))) = pow2 48 * ((v a1 / pow2 22) % pow2 8) + pow2 48 * ((v a2*pow2 4)%pow2 8))
+  = cut (v (a1 >>^ 22ul) = v a1 / pow2 22);
+    Math.Lemmas.pow2_multiplication_modulo_lemma_2 (v a2) 64 4;
+    Math.Lemmas.pow2_lt_compat 60 26; Math.Lemmas.modulo_lemma (v a2) (pow2 60);
+    Math.Lemmas.lemma_mod_plus 0 (v a2) (pow2 4);
+    lemma_div_pow2_lt (v a1) 26 22;
+    cut (v (a2 <<^ 4ul) % pow2 4 = 0);
+    cut (v (a1 >>^ 22ul) < pow2 4);
+    assert_norm(pow2 0 = 1);
+    Math.Lemmas.pow2_plus 26 4;
+    lemma_disjoint_bounded (a1 >>^ 22ul) (a2 <<^ 4ul) 0 4 30;
+    let r = U8.v (uint64_to_uint8 ((a1 >>^ 22ul) |^ (a2 <<^ 4ul))) in
+    cut (r = ((v a1 / pow2 22) + (v a2 * pow2 4)) % pow2 8);
+    lemma_mod_sum_mul (v a2 * pow2 4) (v a1 / pow2 22) 4 8
+
+
+let lemma_b9 (a2:U64.t{v a2 < pow2 26}) (a3:U64.t{v a3 < pow2 26}) : Lemma
+  (pow2 72 * (U8.v (uint64_to_uint8 ((a2 >>^ 20ul) |^ (a3 <<^ 6ul)))) = pow2 72 * ((v a2 / pow2 20) % pow2 8) + pow2 72 * ((v a3*pow2 6)%pow2 8))
+  = cut (v (a2 >>^ 20ul) = v a2 / pow2 20);
+    Math.Lemmas.pow2_multiplication_modulo_lemma_2 (v a3) 64 6;
+    Math.Lemmas.pow2_lt_compat 58 26; Math.Lemmas.modulo_lemma (v a3) (pow2 58);
+    Math.Lemmas.lemma_mod_plus 0 (v a3) (pow2 6);
+    lemma_div_pow2_lt (v a2) 26 20;
+    cut (v (a3 <<^ 6ul) % pow2 6 = 0);
+    cut (v (a2 >>^ 20ul) < pow2 6);
+    assert_norm(pow2 0 = 1);
+    Math.Lemmas.pow2_plus 26 6;
+    lemma_disjoint_bounded (a2 >>^ 20ul) (a3 <<^ 6ul) 0 6 32;
+    let r = U8.v (uint64_to_uint8 ((a2 >>^ 20ul) |^ (a3 <<^ 6ul))) in
+    cut (r = ((v a2 / pow2 20) + (v a3 * pow2 6)) % pow2 8);
+    lemma_mod_sum_mul (v a3 * pow2 6) (v a2 / pow2 20) 6 8
+
+
+
+let lemma_distr_4 a b c d e : Lemma (a * (b+c+d+e) = a * b + a * c + a * d + a * e) = ()
+let lemma_distr_3 a b c d : Lemma (a * (b+c+d) = a * b + a * c + a * d) = ()
+
+let lemma_distr_4_1 b c d e : Lemma (pow2 24 * (b + pow2 8 * c + pow2 16 * d + pow2 24 * e)
+  = pow2 24 * b + pow2 32 * c + pow2 40 * d + pow2 48 * e) =
+    lemma_distr_4 (pow2 24) b (pow2 8 * c) (pow2 16 * d) (pow2 24 * d);
+    Math.Lemmas.pow2_plus 24 8; Math.Lemmas.pow2_plus 24 16; Math.Lemmas.pow2_plus 24 24
+let lemma_distr_4_2 b c d e : Lemma (pow2 48 * (b + pow2 8 * c + pow2 16 * d + pow2 24 * e)
+  = pow2 48 * b + pow2 56 * c + pow2 64 * d + pow2 72 * e) =
+    lemma_distr_4 (pow2 48) b (pow2 8 * c) (pow2 16 * d) (pow2 24 * d);
+    Math.Lemmas.pow2_plus 48 8; Math.Lemmas.pow2_plus 48 16; Math.Lemmas.pow2_plus 48 24
+let lemma_distr_4_3 b c d e : Lemma (pow2 72 * (b + pow2 8 * c + pow2 16 * d + pow2 24 * e)
+  = pow2 72 * b + pow2 80 * c + pow2 88 * d + pow2 96 * e) =
+    lemma_distr_4 (pow2 72) b (pow2 8 * c) (pow2 16 * d) (pow2 24 * d);
+    Math.Lemmas.pow2_plus 72 8; Math.Lemmas.pow2_plus 72 16; Math.Lemmas.pow2_plus 72 24
+let lemma_distr_4_4 b c d : Lemma (pow2 104 * (b + pow2 8 * c + pow2 16 * d)
+  = pow2 104 * b + pow2 112 * c + pow2 120 * d) =
+    lemma_distr_3 (pow2 104) b (pow2 8 * c) (pow2 16 * d);
+    Math.Lemmas.pow2_plus 104 8; Math.Lemmas.pow2_plus 104 16
+
+let lemma_b03a0 (a0:U64.t{v a0 < pow2 26}) (a1:UInt64.t{v a1 < pow2 26}) b0 b1 b2 b3 : Lemma
+  (requires (let open FStar.UInt8 in
+    v b0 = (U64.v a0) % pow2 8
+    /\ v b1 = (U64.v a0 / pow2 8) % pow2 8
+    /\ v b2 = (U64.v a0 / pow2 16) % pow2 8
+    /\ pow2 24 * v b3 = pow2 24 * ((U64.v a0/pow2 24) % pow2 8) + pow2 24 * ((U64.v a1*pow2 2)%pow2 8)))
+  (ensures (let open FStar.UInt8 in
+    v b0 + pow2 8 * v b1 + pow2 16 * v b2 + pow2 24 * v b3 = (U64.v a0) % pow2 32 + pow2 24 * ((U64.v a1*pow2 2)%pow2 8)))
+  = lemma_trunc1305_0 a0
+
+
+#reset-options "--initial_fuel 0 --max_fuel 0 --z3timeout 20"
+
+let lemma_b46a1 (a1:U64.t{v a1 < pow2 26}) (a2:UInt64.t{v a2 < pow2 26}) v3 b4 b5 b6 : Lemma
+  (requires (let open FStar.UInt8 in
+    v3 = pow2 24 * ((U64.v a1*pow2 2)%pow2 8)
+    /\ v b4 = (U64.v a1 / pow2 6) % pow2 8
+    /\ v b5 = (U64.v a1 / pow2 14) % pow2 8
+    /\ pow2 48 * v b6 = pow2 48 * ((U64.v a1 / pow2 22) % pow2 8) + pow2 48 * ((U64.v a2*pow2 4)%pow2 8)))
+  (ensures (let open FStar.UInt8 in
+    v3 + pow2 32 * v b4 + pow2 40 * v b5 + pow2 48 * v b6 = pow2 26 * (U64.v a1 % pow2 30)
+      + pow2 48 * ((U64.v a2*pow2 4)%pow2 8)))
+  = lemma_trunc1305_1 a1; Math.Lemmas.pow2_plus 24 2;
+    Math.Lemmas.distributivity_add_right (pow2 24) (pow2 24 * ((U64.v a1 / pow2 22) % pow2 8)) (pow2 24 * ((U64.v a2*pow2 4)%pow2 8));
+    Math.Lemmas.pow2_plus 24 24;
+    cut (pow2 2 * (v a1 % pow2 30) = ((U64.v a1*pow2 2)%pow2 8) + pow2 8 * U8.v b4 + pow2 16 * U8.v b5 + pow2 24 * ((U64.v a1 / pow2 22) % pow2 8));
+    lemma_distr_4_1 ((U64.v a1*pow2 2)%pow2 8) (U8.v b4) (U8.v b5) ((U64.v a1 / pow2 22) % pow2 8);
+    cut (pow2 24 * (pow2 2 * (v a1 % pow2 30)) = v3 + pow2 32 * U8.v b4 + pow2 40 * U8.v b5
+      + pow2 48 * ((U64.v a1 / pow2 22) % pow2 8));
+    Math.Lemmas.paren_mul_right (pow2 24) (pow2 2) (v a1 % pow2 30)
+
+
+#reset-options "--initial_fuel 0 --max_fuel 0 --z3timeout 20"
+
+let lemma_b79a2 (a2:U64.t{v a2 < pow2 26}) (a3:UInt64.t{v a3 < pow2 26}) v6 b7 b8 b9 : Lemma
+  (requires (let open FStar.UInt8 in
+    v6 = pow2 48 * ((U64.v a2*pow2 4)%pow2 8)
+    /\ v b7 = (U64.v a2 / pow2 4) % pow2 8
+    /\ v b8 = (U64.v a2 / pow2 12) % pow2 8
+    /\ pow2 72 * v b9 = pow2 72 * ((U64.v a2 / pow2 20) % pow2 8) + pow2 72 * ((U64.v a3*pow2 6)%pow2 8)))
+  (ensures (let open FStar.UInt8 in
+    v6 + pow2 56 * v b7 + pow2 64 * v b8 + pow2 72 * v b9 = pow2 52 * (U64.v a2 % pow2 28)
+      + pow2 72 * ((U64.v a3*pow2 6)%pow2 8)))
+  = lemma_trunc1305_2 a2; Math.Lemmas.pow2_plus 48 4;
+    Math.Lemmas.distributivity_add_right (pow2 48) (pow2 48 * ((U64.v a2 / pow2 20) % pow2 8)) (pow2 24 * ((U64.v a3*pow2 6)%pow2 8));
+    Math.Lemmas.pow2_plus 48 24;
+    cut (pow2 4 * (v a2 % pow2 28) = ((U64.v a2*pow2 4)%pow2 8) + pow2 8 * U8.v b7 + pow2 16 * U8.v b8 + pow2 24 * ((U64.v a2 / pow2 20) % pow2 8));
+    lemma_distr_4_2 ((U64.v a2*pow2 4)%pow2 8) (U8.v b7) (U8.v b8) ((U64.v a2 / pow2 20) % pow2 8);
+    cut (pow2 48 * (pow2 4 * (v a2 % pow2 28)) = v6 + pow2 56 * U8.v b7 + pow2 64 * U8.v b8
+      + pow2 72 * ((U64.v a2 / pow2 20) % pow2 8));
+    Math.Lemmas.paren_mul_right (pow2 48) (pow2 4) (v a2 % pow2 28)
+
+
+#reset-options "--initial_fuel 0 --max_fuel 0 --z3timeout 20"
+
+let lemma_b1012a3 (a3:U64.t{v a3 < pow2 26}) v9 b10 b11 b12 : Lemma
+  (requires (let open FStar.UInt8 in
+    v9 = pow2 72 * ((U64.v a3*pow2 6)%pow2 8)
+    /\ v b10 = (U64.v a3 / pow2 2) % pow2 8
+    /\ v b11 = (U64.v a3 / pow2 10) % pow2 8
+    /\ v b12 = ((U64.v a3 / pow2 18) % pow2 8) ))
+  (ensures (let open FStar.UInt8 in
+    v9 + pow2 80 * v b10 + pow2 88 * v b11 + pow2 96 * v b12 = pow2 78 * (U64.v a3 % pow2 26)))
+  = lemma_trunc1305_3 a3; Math.Lemmas.pow2_plus 72 6;
+    cut (pow2 6 * (v a3 % pow2 26) = ((U64.v a3*pow2 6)%pow2 8) + pow2 8 * U8.v b10 + pow2 16 * U8.v b11 + pow2 24 * U8.v b12);
+    lemma_distr_4_3 ((U64.v a3*pow2 6)%pow2 8) (U8.v b10) (U8.v b11) (U8.v b12);
+    cut (pow2 72 * (pow2 6 * (v a3 % pow2 26)) = v9 + pow2 80 * U8.v b10 + pow2 88 * U8.v b11
+      + pow2 96 * U8.v b12);
+    Math.Lemmas.paren_mul_right (pow2 72) (pow2 6) (v a3 % pow2 26)
+
+
+#reset-options "--initial_fuel 0 --max_fuel 0 --z3timeout 20"
+
+let lemma_b1315a4 (a4:U64.t{v a4 < pow2 26}) b13 b14 b15 : Lemma
+  (requires (let open FStar.UInt8 in
+    v b13 = ((U64.v a4)%pow2 8)
+    /\ v b14 = (U64.v a4 / pow2 8) % pow2 8
+    /\ v b15 = (U64.v a4 / pow2 16) % pow2 8))
+  (ensures (let open FStar.UInt8 in
+    pow2 104 * v b13 + pow2 112 * v b14 + pow2 120 * v b15 = pow2 104 * (U64.v a4 % pow2 24)))
+  = lemma_trunc1305_4 a4;
+    lemma_distr_4_4 (U8.v b13) (U8.v b14) (U8.v b15)
+
+let u26 = x:U64.t{v x < pow2 26}
+
+#reset-options "--initial_fuel 0 --max_fuel 0 --z3timeout 20"
+
+val lemma_trunc1305_:
+  a0:u26 -> a1:u26 -> a2:u26 -> a3:u26 -> a4:u26 ->
+  b0:U8.t -> b1:U8.t -> b2:U8.t -> b3:U8.t -> b4:U8.t -> b5:U8.t -> b6:U8.t -> b7:U8.t ->
+  b8:U8.t -> b9:U8.t -> b10:U8.t -> b11:U8.t -> b12:U8.t -> b13:U8.t -> b14:U8.t -> b15:U8.t ->
+  Lemma (requires (let open FStar.UInt8 in
+    v b0 = (U64.v a0) % pow2 8
+    /\ v b1 = (U64.v a0 / pow2 8) % pow2 8
+    /\ v b2 = (U64.v a0 / pow2 16) % pow2 8
+    /\ pow2 24 * v b3 = pow2 24 * ((U64.v a0/pow2 24) % pow2 8) + pow2 24 * ((U64.v a1*pow2 2)%pow2 8)
+    /\ v b4 = (U64.v a1 / pow2 6) % pow2 8
+    /\ v b5 = (U64.v a1 / pow2 14) % pow2 8
+    /\ pow2 48 * v b6 = pow2 48 * ((U64.v a1 / pow2 22) % pow2 8) + pow2 48 * ((U64.v a2*pow2 4)%pow2 8)
+    /\ v b7 = (U64.v a2 / pow2 4) % pow2 8
+    /\ v b8 = (U64.v a2 / pow2 12) % pow2 8
+    /\ pow2 72 * v b9 = pow2 72 * ((U64.v a2 / pow2 20) % pow2 8) + pow2 72 * ((U64.v a3*pow2 6)%pow2 8)
+    /\ v b10 = (U64.v a3 / pow2 2) % pow2 8
+    /\ v b11 = (U64.v a3 / pow2 10) % pow2 8
+    /\ v b12 = ((U64.v a3 / pow2 18) % pow2 8)
+    /\ v b13 = ((U64.v a4)%pow2 8)
+    /\ v b14 = (U64.v a4 / pow2 8) % pow2 8
+    /\ v b15 = (U64.v a4 / pow2 16) % pow2 8 ))
+        (ensures  (U8 (v (b0) + pow2 8 * v (b1) + pow2 16 * v (b2) + pow2 24 * v (b3)
+  + pow2 32 * v (b4) + pow2 40 * v (b5) + pow2 48 * v (b6) + pow2 56 * v (b7)
+  + pow2 64 * v (b8) + pow2 72 * v (b9) + pow2 80 * v (b10) + pow2 88 * v (b11)
+  + pow2 96 * v (b12) + pow2 104 * v (b13) + pow2 112 * v (b14) + pow2 120 * v (b15))
+            = v a0 + pow2 26 * v a1 + pow2 52 * v a2 + pow2 78 * v a3 + pow2 104 * (v a4 % pow2 24)))
+
+let lemma_sub a b c : Lemma (requires (a + b = c)) (ensures (a = a + b - b /\ a = c - b)) = ()
+let lemma_paren a b c d : Lemma (a + (b + c + d) = a + b + c + d) = ()
+let lemma_sum_ a b c d e f g h : Lemma ((a-b)+((b+c)-d)+((d+e)-f)+(f+g)+h=a+c+e+g+h) = ()
+let lemma_sum' b0 b1 b2 b3 b4 b5 b6 b7 b8 b9 b10 b11 b12 b13 b14 b15 : Lemma
+  (b0+b1+b2+b3+b4+b5+b6+b7+b8+b9+b10+b11+b12+b13+b14+b15 = (b0+b1+b2+b3)+(b4+b5+b6)+(b7+b8+b9)+(b10+b11+b12)+(b13+b14+b15)) = ()
+
+#reset-options "--initial_fuel 0 --max_fuel 0 --z3timeout 100"
+
+let lemma_trunc1305_ a0 a1 a2 a3 a4 b0 b1 b2 b3 b4 b5 b6 b7 b8 b9 b10 b11 b12 b13 b14 b15 =
+  lemma_b3 a0 a1;
+  lemma_b6 a1 a2;
+  lemma_b9 a2 a3;
+  let open FStar.UInt8 in
+  lemma_distr_4_1 ((U64.v a1*pow2 2)%pow2 8) (v b4) (v b5) ((U64.v a1 / pow2 22) % pow2 8);
+  lemma_distr_4_2 ((U64.v a2*pow2 4)%pow2 8) (v b7) (v b8) ((U64.v a2 / pow2 20) % pow2 8);
+  lemma_distr_4_3 ((U64.v a3*pow2 6)%pow2 8) (v b10) (v b11) (v b12);
+  let v3 = pow2 24 * ((U64.v a1*pow2 2)%pow2 8) in
+  let v6 = pow2 48 * ((U64.v a2*pow2 4)%pow2 8) in
+  let v9 = pow2 72 * ((U64.v a3*pow2 6)%pow2 8) in
+  let b03 = (v b0 + pow2 8 * v b1 + pow2 16 * v b2 + pow2 24 * v b3) in
+  let b46 = pow2 32 * v (b4) + pow2 40 * v (b5) + pow2 48 * v (b6) in
+  let b79 = pow2 56 * v (b7) + pow2 64 * v (b8) + pow2 72 * v (b9) in
+  let b1012 = pow2 80 * v (b10) + pow2 88 * v (b11) + pow2 96 * v (b12) in
+  let b1315 = pow2 104 * v (b13) + pow2 112 * v (b14) + pow2 120 * v (b15) in
+  lemma_b03a0 a0 a1 b0 b1 b2 b3;
+  lemma_b46a1 a1 a2 (v3) b4 b5 b6;
+  lemma_paren v3 (pow2 32 * v (b4)) (pow2 40 * v (b5)) (pow2 48 * v (b6));
+  cut ( pow2 26 * (U64.v a1 % pow2 30) + v6 = v3 + b46);
+  lemma_b79a2 a2 a3 (v6) b7 b8 b9;
+  lemma_paren v6 (pow2 56 * v (b7)) (pow2 64 * v (b8)) (pow2 72 * v (b9));
+  cut ( pow2 52 * (U64.v a2 % pow2 28) + v9 = v6 + b79);
+  lemma_b1012a3 a3 (v9) b10 b11 b12;
+  lemma_paren v9 (pow2 80 * v (b10)) (pow2 88 * v (b11)) (pow2 96 * v (b12));
+  cut ( pow2 78 * (U64.v a3 % pow2 26) = v9 + b1012);
+  lemma_b1315a4 a4 b13 b14 b15;
+  cut ( pow2 104 * (U64.v a4 % pow2 24) = b1315);
+  lemma_sub ((U64.v a0) % pow2 32) v3 b03;
+  let open FStar.UInt64 in
+  cut ((v a0 % pow2 32) = b03 - v3);
+  lemma_sub (pow2 26 * ((U64.v a1) % pow2 30)) v6 (v3 + b46);
+  lemma_sub (pow2 52 * ((U64.v a2) % pow2 28)) v9 (v6 + b79);
+  cut (pow2 26 * (v a1 % pow2 30) = (v3 + b46) - v6);
+  cut (pow2 52 * (v a2 % pow2 28) = (v6 + b79) - v9);
+  cut ((v a0 % pow2 32)
+            + pow2 26 * (v a1 % pow2 30)
+            + pow2 52 * (v a2 % pow2 28)
+            + pow2 78 * (v a3 % pow2 26)
+            + pow2 104 * (v a4 % pow2 24) = (b03 - v3) + ((v3 + b46) - v6) + ((v6 + b79) - v9)
+              + (v9 + b1012) + b1315);
+   lemma_sum_ b03 v3 b46 v6 b79 v9 b1012 b1315;
+   let open FStar.UInt8 in
+   lemma_sum' (v b0) (v b1) (v b2) (v b3) (v b4) (v b5) (v b6) (v b7) (v b8) (v b9) (v b10) (v b11) (v b12) (v b13) (v b14) (v b15);
+   let open FStar.UInt64 in
+   Math.Lemmas.pow2_lt_compat 32 26; Math.Lemmas.pow2_lt_compat 30 26;
+   Math.Lemmas.pow2_lt_compat 28 26; Math.Lemmas.modulo_lemma (v a0) (pow2 32);
+   Math.Lemmas.modulo_lemma (v a1) (pow2 30); Math.Lemmas.modulo_lemma (v a2) (pow2 28);
+   Math.Lemmas.modulo_lemma (v a3) (pow2 26)
+
+
+#reset-options "--initial_fuel 0 --max_fuel 0 --z3timeout 20"
+
+let lemma_mult_le_left (a:nat) (b:nat) (c:nat) : Lemma (requires (b <= c)) (ensures (a * b <= a * c)) = ()
+
+val lemma_eval_mod: a0:u26 -> a1:u26 -> a2:u26 -> a3:u26 -> a4:u26 -> Lemma
+  ((v a0 + pow2 26 * v a1 + pow2 52 * v a2 + pow2 78 * v a3 + pow2 104 * v a4) % pow2 128
+    = v a0 + pow2 26 * v a1 + pow2 52 * v a2 + pow2 78 * v a3 + (pow2 104 * (v a4 % pow2 24)))
+let lemma_eval_mod a0 a1 a2 a3 a4 =
+  Math.Lemmas.lemma_mod_plus_distr_l (pow2 104 * v a4) (v a0 + pow2 26 * v a1 + pow2 52 * v a2 + pow2 78 * v a3) (pow2 128);
+  let r' = v a0 + pow2 26 * v a1 + pow2 52 * v a2 + pow2 78 * v a3 in
+  let r = (v a0 + pow2 26 * v a1 + pow2 52 * v a2 + pow2 78 * v a3 + pow2 104 * v a4) % pow2 128 in
+  let r'' = (v a0 + pow2 26 * v a1 + pow2 52 * v a2 + pow2 78 * v a3 + pow2 104 * (v a4 % pow2 24)) in
+  cut (r = (((pow2 104 * v a4)%pow2 128) + r') % pow2 128);
+  Math.Lemmas.pow2_multiplication_modulo_lemma_2 (v a4) 128 104;
+  cut ((pow2 104 * v a4) % pow2 128 = pow2 104 * (v a4 % pow2 24));
+  cut (r = r'' % pow2 128);
+  lemma_mult_le_left (pow2 26) (v a1) (pow2 26 - 1);
+  lemma_mult_le_left (pow2 52) (v a2) (pow2 26 - 1);
+  lemma_mult_le_left (pow2 78) (v a3) (pow2 26 - 1);
+  lemma_mult_le_left (pow2 104) (v a4 % pow2 24) (pow2 24 - 1);
+  assert_norm ((pow2 26 - 1) + pow2 26 * (pow2 26 - 1) + pow2 52 * (pow2 26 - 1) + pow2 78 * (pow2 26 - 1) + (pow2 104 * ((pow2 24 - 1))) < pow2 128);
+  Math.Lemmas.modulo_lemma ( v a0 + pow2 26 * v a1 + pow2 52 * v a2 + pow2 78 * v a3 + (pow2 104 * (v a4 % pow2 24))) (pow2 128)
+
 
 val lemma_trunc1305: hb:HyperStack.mem ->
   b:Buffer.buffer U8.t{live hb b /\ length b = 16} ->
@@ -572,23 +1074,12 @@ val lemma_trunc1305: hb:HyperStack.mem ->
         (ensures  ((Crypto.Symmetric.Poly1305.Bigint.eval ha a 5) % pow2 128
           = little_endian (as_seq hb b)))
 
-let lemma_b3 (a0:U64.t{v a0 < pow2 26}) (a1:U64.t{v a1 < pow2 26}) : Lemma
-  (U8.v (uint64_to_uint8 ((a0 >>^ 24ul) |^ (a1 <<^ 2ul))) = ((v a0 / pow2 24) % pow2 8) + ((v a1*pow2 2)%pow2 8))
-  = admit()
 
-
-let lemma_b6 (a1:U64.t{v a1 < pow2 26}) (a2:U64.t{v a2 < pow2 26}) : Lemma
-  (U8.v (uint64_to_uint8 ((a1 >>^ 22ul) |^ (a2 <<^ 4ul))) = ((v a1 / pow2 22) % pow2 8) + ((v a2*pow2 4)%pow2 8))
-  = admit()
-
-
-let lemma_b9 (a2:U64.t{v a2 < pow2 26}) (a3:U64.t{v a3 < pow2 26}) : Lemma
-  (U8.v (uint64_to_uint8 ((a2 >>^ 20ul) |^ (a3 <<^ 6ul))) = ((v a2 / pow2 20) % pow2 8) + ((v a3*pow2 6)%pow2 8))
-  = admit()
-
+#reset-options "--initial_fuel 0 --max_fuel 0 --z3timeout 20"
 
 let lemma_trunc1305 hb b ha a =
   lemma_little_endian_16 hb b;
+  lemma_eval_5 ha a;
   lemma_norm_5 ha a;
   let a0 = get ha a 0 in let a1 = get ha a 1 in let a2 = get ha a 2 in let a3 = get ha a 3 in
   let a4 = get ha a 4 in
@@ -602,14 +1093,6 @@ let lemma_trunc1305 hb b ha a =
   let p96 = pow2 96 in let p104 = pow2 104 in let p112 = pow2 112 in let p120 = pow2 120 in
   lemma_b3 a0 a1;
   lemma_b6 a1 a2;
-  lemma_b9 a2 a3; admit()
-  (* assume (U8.v b3 = ((v a0 / p24) % p8) + ((v a1*pow2 2)%p8)); admit() *)
-
-  (* let le =  v (b0) + pow2 8 * v (b1) + pow2 16 * v (b2) + pow2 24 * v (b3) *)
-  (* + pow2 32 * v (b4) + pow2 40 * v (b5) + pow2 48 * v (b6) + pow2 56 * v (b7) *)
-  (* + pow2 64 * v (b8) + pow2 72 * v (b9) + pow2 80 * v (b10) + pow2 88 * v (b11) *)
-  (* + pow2 96 * v (b12) + pow2 104 * v (b13) + pow2 112 * v (b14) + pow2 120 * v (b15) in *)
-  
-
-  (* cut (le = ((v a0 % p8) + p8 * ((v a0 / p8) % p8) + p16 * ((v a0 / p16)%p8) + p24*((v a0/p24)%p8) *)
-  (*   + p32*((v a1)/pow2 6)%p8) + p40*((v a1/pow2 14)%p8) + p48*((v a1/pow2 22)%p8) + p24*((v a0/p24)%p8) *)
+  lemma_b9 a2 a3;
+  lemma_trunc1305_ a0 a1 a2 a3 a4 b0 b1 b2 b3 b4 b5 b6 b7 b8 b9 b10 b11 b12 b13 b14 b15;
+  lemma_eval_mod a0 a1 a2 a3 a4
